Parser proof: Sketch for next

theories/CeresParserRoundtrip.v
@@ -31,29 +31,52 @@ Inductive comment : string -> Prop :=
 (* TODO *)
 .
 
-Inductive atom_string (s1 s : string) : Prop :=
-(* TODO: s1 is made of atom characters and s does not start with an atom character *)
+Inductive atom_string (s1 : string) : Prop :=
+(* TODO: s1 is made of atom characters *)
+.
+
+Inductive after_atom_string (s : string) (more : bool) : Prop :=
+ (* TODO: s does not start with an atom character *)
 .
 
 Inductive string_string (s0 : string) (s1 : string) : Prop :=
 (* TODO: s1 = "s0" *)
 .
 
-(* Lexer relation: [token_string ts s] if the string [s] can be split into tokens [ts].
+(* Lexer relation: [token_string more ts s] if the string [s] can be split into tokens [ts].
    - Handling of spaces and comments.
    - Corner cases for spaces around atoms (["ab"] should not be parsed as ["a"] then ["b"]).
+   - [more] is true if the last token is an [Token.Atom] and there are no more
+     characters after it, in which case we need to be careful to append something.
  *)
-Inductive token_string : list Token.t -> string -> Prop :=
-| token_string_nil : token_string [] ""
-| token_string_spaces ts ws s : whitespaces ws -> token_string ts s -> token_string ts (ws ++ s)
-| token_string_comment ts c s : comment c -> token_string ts s -> token_string ts (c ++ s)
-| token_string_open ts s : token_string ts s -> token_string (Token.Open :: ts) ("(" :: s)
-| token_string_close ts s : token_string ts s -> token_string (Token.Close :: ts) (")" :: s)
+Inductive token_string (more : bool) : list Token.t -> string -> Prop :=
+| token_string_nil : token_string more [] ""
+| token_string_spaces ts ws s
+  : whitespaces ws -> token_string more ts s -> token_string more ts (ws ++ s)
+| token_string_comment ts c s
+  : comment c -> token_string more ts s -> token_string more ts (c ++ s)
+| token_string_open ts s
+  : token_string more ts s -> token_string more (Token.Open :: ts) ("(" :: s)
+| token_string_close ts s
+  : token_string more ts s -> token_string more (Token.Close :: ts) (")" :: s)
 | token_string_atom ts s1 s
-  : atom_string s1 s -> token_string ts s -> token_string (Token.Atom s1 :: ts) (s1 ++ s)
+  : atom_string s1 -> after_atom_string s more ->
+    token_string more ts s -> token_string more (Token.Atom s1 :: ts) (s1 ++ s)
 | token_string_string ts s0 s1 s
-  : string_string s0 s1 -> token_string ts s -> token_string (Token.Str s0 :: ts) (s1 ++ s)
+  : string_string s0 s1 -> token_string more ts s -> token_string more (Token.Str s0 :: ts) (s1 ++ s)
 .
+Hint Constructors token_string : core.
+
+Inductive more_ok : bool -> string -> Prop :=
+| more_ok_false s : more_ok false s
+| more_ok_true c s : (* TODO c is not an Atom character *) more_ok true (c :: s)
+.
+Hint Constructors more_ok : core.
+
+Lemma more_ok_nil_inv more : more_ok more "" -> more = false.
+Proof.
+  inversion 1; reflexivity.
+Qed.
 
 (* * Parser *)
 
@@ -77,10 +100,171 @@ Inductive sexp_tokens : sexp -> list Token.t -> Prop :=
 
 Definition list_sexp_tokens := list_tokens sexp_tokens.
 
+(* * Lemmas *)
+
+Lemma string_app_assoc (s0 s1 s2 : string)
+  : ((s0 ++ s1) ++ s2 = s0 ++ (s1 ++ s2))%string.
+Proof.
+  induction s0; cbn; [ auto | rewrite IHs0; auto ].
+Qed.
+
+Lemma after_atom_string_open_app s more :
+  after_atom_string (s ++ "(") more.
+Proof.
+Admitted.
+
+Lemma token_string_open_app more ts s :
+  token_string more ts s ->
+  token_string false (ts ++ [Token.Open]) (s ++ "(").
+Proof.
+  induction 1; cbn; try rewrite (string_app_assoc _ _ "("%string); eauto.
+  apply token_string_atom; auto.
+  apply after_atom_string_open_app.
+Qed.
+
+(* * Parser state *)
+
+Inductive stack_tokens : list symbol -> list Token.t -> Prop :=
+| stack_tokens_nil : stack_tokens [] []
+| stack_tokens_open p us ts
+  : stack_tokens us ts ->
+    stack_tokens (Open p :: us) (ts ++ [Token.Open])
+| stack_tokens_sexp e us ts ts0
+  : sexp_tokens e ts0 ->
+    stack_tokens us ts ->
+    stack_tokens (Exp e :: us) (ts ++ ts0)
+.
+Hint Constructors stack_tokens : core.
+
+Definition escape_to_string (e : escape) : string :=
+  match e with
+  | EscBackslash => "\"
+  | EscNone => ""
+  end.
+
+Definition nonewline (s : string) : Prop.
+Admitted.
+
+Inductive partial_token_string : partial_token -> string -> Prop :=
+| partial_token_string_NoToken
+  : partial_token_string NoToken ""
+| partial_token_string_SimpleToken p s
+  : partial_token_string (SimpleToken p s) s
+| partial_token_string_StrToken p tok e
+  : partial_token_string (StrToken p tok e) ("""" :: string_reverse tok ++ escape_to_string e)
+| partial_token_string_Comment s
+  : nonewline s ->
+    partial_token_string Comment (";" :: s)
+.
+Hint Constructors partial_token_string : core.
+
+(* Invariant on the parsed prefix *)
+Inductive parser_state_string (i : parser_state) : string -> Prop :=
+| parser_state_string_mk more ts00 ts01 s0 s1
+  : token_string more (ts00 ++ ts01) s0 ->
+    more_ok more s1 ->
+    list_sexp_tokens (parser_done i) ts00 ->
+    stack_tokens (parser_stack i) ts01 ->
+    partial_token_string (parser_cur_token i) s1 ->
+    parser_state_string i (s0 ++ s1)
+.
+
+Definition on_right {A B} (x : A + B) (P : B -> Prop) : Prop :=
+  match x with
+  | inl _ => True
+  | inr b => P b
+  end.
+
+Ltac match_ascii :=
+  repeat
+    match goal with
+    | [ |- context E [ eqb_ascii ?x ?y ] ] =>
+      destruct (eqb_eq_ascii' x y)
+    end.
+
+Lemma string_app_nil_r (s : string) : (s ++ "")%string = s.
+Proof.
+  induction s; [ auto | cbn; rewrite IHs; auto ].
+Qed.
+
+Lemma next_sound i s p c
+  : parser_state_string i s ->
+    on_right (next i p c) (fun i' =>
+      parser_state_string i' (s ++ c :: "")).
+Proof.
+  intros [more ts00 ts01 s0 s1 Hs0 Hmore Hdone Hstack Hcur].
+  unfold next.
+  destruct Hcur as [ | p1' s1' | p1 tok e | s1' Hs ].
+  - (* NoToken *)
+    unfold next'.
+    apply more_ok_nil_inv in Hmore; subst more.
+    rewrite string_app_nil_r.
+    match_ascii; cbn.
+    + (* "(" *)
+      rewrite <- (string_app_nil_r (s0 ++ "(")).
+      apply parser_state_string_mk
+        with (more := false) (ts00 := ts00) (ts01 := ts01 ++ [Token.Open]);
+        cbn; auto.
+      rewrite app_assoc; eapply token_string_open_app; eauto.
+    + (* ")" *)
+      admit.
+    + (* """" (double quote char) *)
+      apply parser_state_string_mk
+        with (more := false) (ts00 := ts00) (ts01 := ts01);
+        cbn; auto.
+      constructor.
+    + (* ";" *)
+      apply parser_state_string_mk
+        with (more := false) (ts00 := ts00) (ts01 := ts01);
+        cbn; auto.
+      constructor.
+      admit.
+    + (* else *)
+      destruct (is_whitespace _) eqn:Hws; cbn.
+      * rewrite <- (string_app_nil_r (s0 ++ y :: "")).
+        apply parser_state_string_mk
+          with (more := false) (ts00 := ts00) (ts01 := ts01);
+          cbn; auto.
+        admit.
+      * admit.
+  - (* SimpleToken *)
+    unfold next'.
+    match_ascii; cbn.
+    + (* "(" *)
+      rewrite <- (string_app_nil_r (_ ++ "(")).
+      apply parser_state_string_mk
+        with (more := false) (ts00 := ts00) (ts01 := ts01 ++ [Token.Open]);
+        cbn; auto.
+      * rewrite app_assoc; apply token_string_open_app with (more := true); eauto.
+        admit.
+      * admit.
+      * admit.
+    + (* ")" *)
+      admit.
+    + (* """" *)
+      admit.
+    + (* ";" *)
+      admit.
+    + (* else *)
+      admit.
+  - (* StrToken *)
+    admit.
+  - (* Comment *)
+    admit.
+Abort.
+
+(*
+Lemma _parse_sexps_sound (s : string) (es : list sexp)
+  : parse_sexps_ s = inr es ->
+    exists ts,
+      list_sexp_tokens es ts /\ token_string ts s.
+Proof.
+*)
+
 (* If the parser succeeds, then the expressions relate to the above *)
 Theorem parse_sexps_sound (s : string) (es : list sexp)
   : parse_sexps s = inr es ->
-    exists ts,
-      list_sexp_tokens es ts /\ token_string ts s.
+    exists more ts,
+      list_sexp_tokens es ts /\ token_string more ts s.
 Proof.
 Abort.
